pk_dh.v
@@ -31,11 +31,15 @@ Definition pk_dh_mk_session_key_impl rl : val :=
 
 Variable N : namespace.
 
+Definition pk_dh_init : val := λ: "c",
+  pk_auth_init N "c" pk_dh_mk_key_share_impl (pk_dh_mk_session_key_impl Init).
+
+Definition pk_dh_resp : val := λ: "c",
+  pk_auth_resp N "c" pk_dh_mk_key_share_impl (pk_dh_mk_session_key_impl Resp).
+
+#[local]
 Program Instance PK_DH : PK := {
-  is_priv_key n kI kR := (
-    □ (pterm n ↔ ▷ False) ∧
-    □ (∀ s, dh_pred n s ↔ ▷ corruption kI kR)
-  )%I;
+  is_priv_key n kI kR := dh_seed (λ _, corruption kI kR) n;
 
   mk_key_share := pk_dh_mk_key_share;
   mk_key_share_impl := pk_dh_mk_key_share_impl;
@@ -55,13 +59,11 @@ move=> n; rewrite sterm_TExp /= sterm_TInt. apply: anti_symm.
 Qed.
 
 Next Obligation.
-iIntros "%nI %kI %kR #s_nI [#p_nI #dh]".
-rewrite /pk_dh_mk_key_share /secret_of pterm_TExp1 sterm_TInt.
-iModIntro. iSplit.
-- iIntros "(_ & _ & #[contra|p_sI])".
-  + iDestruct ("p_nI" with "contra") as ">[]".
-  + iApply "dh". by eauto.
-- iIntros "#fail". do !iSplit => //. iRight. by iApply "dh".
+iIntros "%nI %kI %kR #s_nI #dh".
+rewrite /pk_dh_mk_key_share /secret_of. iModIntro. iSplit.
+- iIntros "#p_sI".
+  by iPoseProof (dh_seed_elim1 with "dh p_sI") as "H".
+- iIntros "#fail". iApply dh_pterm_TExp; eauto. by rewrite sterm_TInt.
 Qed.
 
 Next Obligation.
@@ -77,22 +79,96 @@ Qed.
 Next Obligation.
 iIntros "%E %kI %kR %Φ _ post". rewrite /pk_dh_mk_key_share_impl.
 wp_pures. wp_bind (mknonce _).
-iApply (wp_mknonce _ (λ _, False)%I (λ _, corruption kI kR)).
+iApply (wp_mknonce _ (λ _, False)%I (dh_publ (λ _, corruption kI kR))).
 iIntros "%n #s_n #p_n #dh token". wp_pures.
 wp_bind (tint _). iApply wp_tint.
 wp_bind (tgroup _). iApply wp_tgroup.
 wp_bind (texp _ _). iApply wp_texp. rewrite Spec.texpA.
 wp_pures. iModIntro. iApply "post".
 rewrite bi.intuitionistic_intuitionistically.
-iFrame. iSplit => //. iSplit => //. iModIntro.
-iIntros "%t". iSpecialize ("dh" $! t).
-by rewrite bi.intuitionistic_intuitionistically.
+iFrame. by do !iSplit => //.
 Qed.
 
 Next Obligation.
 iIntros "%E %rl %n %s %Φ _ post".
 rewrite /pk_dh_mk_session_key_impl.
 wp_pures. iApply wp_texp. by iApply "post".
+Qed.
+
+Lemma pk_dh_session_key_elim kI kR kS :
+  session_key N kI kR kS -∗
+  pterm kS →
+  ◇ False.
+Proof.
+iIntros "(%nI & %nR & -> & #priv_nI & #priv_nR & _)".
+rewrite /= /pk_dh_mk_session_key /pk_dh_mk_key_share Spec.texpA.
+iIntros "#p_kS".
+iDestruct (dh_seed_elim2 with "priv_nI p_kS") as "[>p_sI >contra]".
+by iDestruct (dh_seed_elim0 with "priv_nR contra") as ">[]".
+Qed.
+
+Lemma wp_pk_dh_init c kI kR E :
+  ↑cryptisN ⊆ E →
+  ↑N ⊆ E →
+  channel c -∗
+  ctx N -∗
+  pterm (TKey Enc kI) -∗
+  pterm (TKey Enc kR) -∗
+  {{{ True }}}
+    pk_dh_init c (TKey Dec kI) (TKey Enc kI) (TKey Enc kR) @ E
+  {{{ (okS : option term), RET repr okS;
+      if okS is Some kS then
+        sterm kS ∗
+        (corruption kI kR ∨
+         □ (pterm kS → ◇ False) ∗
+         session_key_token N Init kS ∗
+         session_key N kI kR kS)
+      else True
+  }}}.
+Proof.
+iIntros "% % #chan_c #ctx #p_ekI #p_ekR %Ψ !> _ post".
+rewrite /pk_dh_init; wp_pures.
+iApply (wp_pk_auth_init with "chan_c ctx"); eauto.
+iIntros "!> %okS". case: okS => [kS|]; last first.
+  by iApply ("post" $! None).
+iIntros "[#s_kS kSP]". iApply ("post" $! (Some kS)).
+iSplitR => //.
+iDestruct "kSP" as "[fail|[token #key]]"; eauto.
+iRight. iFrame. iSplit => //. iModIntro.
+by iApply pk_dh_session_key_elim.
+Qed.
+
+Lemma wp_pk_dh_resp c kR E :
+  ↑cryptisN ⊆ E →
+  ↑N ⊆ E →
+  channel c -∗
+  ctx N -∗
+  pterm (TKey Enc kR) -∗
+  {{{ True }}}
+    pk_dh_resp c (TKey Dec kR) (TKey Enc kR) @ E
+  {{{ (res : option (term * term)), RET repr res;
+      if res is Some (pkI, kS) then ∃ kI,
+        ⌜pkI = TKey Enc kI⌝ ∧
+        pterm pkI ∧
+        sterm kS ∧
+        (corruption kI kR ∨
+         □ (pterm kS → ◇ False) ∗
+         session_key_token N Resp kS ∗
+         session_key N kI kR kS)
+      else True
+  }}}.
+Proof.
+iIntros "% % #chan_c #ctx #p_ekR %Ψ !> _ post".
+rewrite /pk_dh_resp; wp_pures.
+iApply (wp_pk_auth_resp with "chan_c ctx"); eauto.
+iIntros "!> %res". case: res => [[pkI kS]|]; last first.
+  by iApply ("post" $! None).
+iIntros "(%kI & -> & #p_pkI & #s_kS & kSP)".
+iApply ("post" $! (Some (TKey Enc kI, kS))). iExists kI.
+do 3!iSplitR => //.
+iDestruct "kSP" as "[fail|[token #key]]"; eauto.
+iRight. iFrame. iSplit => //. iModIntro.
+by iApply pk_dh_session_key_elim.
 Qed.
 
 End PKDH.
